---
title: "Homework 2"
author: "Matthew Smith"
date: "10/25/2018"
output:
  html_document:
    self_contained: yes
    toc: true
---
<!--
%\VignetteEngine{knitr::rmarkdown}
%\VignetteIndexEntry{Basis Expansion and LASSO}
-->

# 1. CASL Page 117, Question 7?


# 2. CASL Page 200, Question 3
By the Definition in Section 7.4 (Equation 7.25), a function $f:\mathbb{R}^p\to\mathbb{R}$ is
*convex* if $\forall b_1, b_2 \in \mathbb{R}^p$ and $\forall t \in [0,1]$, we have
$$
f(tb_1 + (1-t)b_2) \leq tf(b_1) + (1-t)f(b_2).
$$
If $f,g:\mathbb{R}^p\to\mathbb{R}$ are both convex, and $h = f + g$, then
$\forall b_1, b_2 \in \mathbb{R}^p$ and $\forall t \in [0,1]$,
$$
\begin{array}{rcll}
h(tb_1 + (1-t)b_2) & = & (f+g)(tb_1 + (1-t)b_2)\\
 & = & f(tb_1 + (1-t)b_2) + g(tb_1 + (1-t)b_2)\\
 & \leq & tf(b_1) + (1-t)f(b_2) + g(tb_1 + (1-t)b_2)\\
 & \leq & tf(b_1) + (1-t)f(b_2) + tg(b_1) + (1-t)g(b_2)\\
 & = & tf(b_1) + tg(b_1) + (1-t)f(b_2) + (1-t)g(b_2)\\
 & = & t(f+g)(b_1) + (1-t)(f+g)(b_2)\\
 & = & th(b_1) + (1-t)(f+g)(b_2).\\
\end{array}
$$
Thus $h(tb_1 + (1-t)b_2) \leq th(b_1) + (1-t)(f+g)(b_2)$ $\forall b_1, b_2 \in \mathbb{R}^p$ and
$\forall t \in [0,1]$. So, if $f$ and $g$ are both convex functions, then their sum $h=f+g$ is as
well.


# 3. CASL Page 200, Question 4
First we will show that the absolute value function is convex. We will use the above definition for
convex functions. Since $t\in[0,1]$, $t$ and $1-t$ are both non-negative. This means,
$\forall x \in \mathbb{R}$, $\lvert tx \rvert = t \lvert x \rvert$ and
$\lvert (1-t)x \rvert = (1-t) \lvert x \rvert$. The absolute value function also follows the
*Triangle Inequality*: $\forall x,y \in \mathbb{R}$,
$\lvert x+y \rvert \leq \lvert x \rvert + \lvert y \rvert$. Then, $\forall x,y \in \mathbb{R}$ and
$\forall t \in [0,1]$,
$$
\begin{array}{rcll}
\lvert tx + (1-t)y \rvert & \leq & \lvert tx \rvert + \lvert (1-ty) \vert\\
 & = & t \lvert x \rvert + (1-t) \lvert y \rvert.\\
\end{array}
$$
By definition, this means that the absolute value function is convex.

In the previous question, we showed that the sum of two convex functions is also convex. Using
induction, we can show that *any* finite sum of $p$ convex functions is also convex. The above proof
would work both as the base case and the induction step.

The $\ell_1$-norm is defined as
$\lvert\lvert \vec{x} \rvert\rvert_1 = \sum_{i=1}^p \lvert x_i \rvert$, $\forall x \in \mathbb{R}^p$.
Since each $\lvert x_i \rvert$ is a convex function, the sum of all these convex absolute value
functions is also convex. Then, the $\ell_1$-norm is convex.


# 4. CASL Page 200, Question 5


# 5. CASL Page 200, Question 6




